rocq/uint256/theories/BarrettStaticChecks.v
@@ -88,6 +88,10 @@ Example reciprocal_1_65_pre_product_word_shift :
   Bar.pre_product_word_shift Bar.addmod_reciprocal_1_65 = 0%nat.
 Proof. static_check. Qed.
 
+Example reciprocal_1_65_post_product_bit_shift :
+  Bar.post_product_bit_shift Bar.addmod_reciprocal_1_65 = 0%nat.
+Proof. static_check. Qed.
+
 Example reciprocal_65_129_bits :
   Bar.reciprocal_bits Bar.addmod_reciprocal_65_129 = 193%nat.
 Proof. static_check. Qed.
@@ -98,6 +102,10 @@ Proof. static_check. Qed.
 
 Example reciprocal_65_129_pre_product_word_shift :
   Bar.pre_product_word_shift Bar.addmod_reciprocal_65_129 = 1%nat.
+Proof. static_check. Qed.
+
+Example reciprocal_65_129_post_product_bit_shift :
+  Bar.post_product_bit_shift Bar.addmod_reciprocal_65_129 = 0%nat.
 Proof. static_check. Qed.
 
 Example reciprocal_129_193_bits :
@@ -112,6 +120,10 @@ Example reciprocal_129_193_pre_product_word_shift :
   Bar.pre_product_word_shift Bar.addmod_reciprocal_129_193 = 2%nat.
 Proof. static_check. Qed.
 
+Example reciprocal_129_193_post_product_bit_shift :
+  Bar.post_product_bit_shift Bar.addmod_reciprocal_129_193 = 0%nat.
+Proof. static_check. Qed.
+
 Example reciprocal_193_256_bits :
   Bar.reciprocal_bits Bar.addmod_reciprocal_193_256 = 65%nat.
 Proof. static_check. Qed.
@@ -122,6 +134,10 @@ Proof. static_check. Qed.
 
 Example reciprocal_193_256_pre_product_word_shift :
   Bar.pre_product_word_shift Bar.addmod_reciprocal_193_256 = 3%nat.
+Proof. static_check. Qed.
+
+Example reciprocal_193_256_post_product_bit_shift :
+  Bar.post_product_bit_shift Bar.addmod_reciprocal_193_256 = 0%nat.
 Proof. static_check. Qed.
 
 Example reciprocal_bits :
@@ -136,6 +152,10 @@ Example reciprocal_input_words :
   Bar.input_words Bar.addmod_reciprocal = 5%nat.
 Proof. static_check. Qed.
 
+Example reciprocal_post_product_bit_shift :
+  Bar.post_product_bit_shift Bar.addmod_reciprocal = 0%nat.
+Proof. static_check. Qed.
+
 End Addmod.
 
 Module Mulmod.
@@ -148,12 +168,20 @@ Example reciprocal_1_65_max_denominator_bits :
   Bar.max_denominator_bits Bar.mulmod_reciprocal_1_65 = 65%nat.
 Proof. static_check. Qed.
 
+Example reciprocal_1_65_post_product_bit_shift :
+  Bar.post_product_bit_shift Bar.mulmod_reciprocal_1_65 = 0%nat.
+Proof. static_check. Qed.
+
 Example reciprocal_65_129_bits :
   Bar.reciprocal_bits Bar.mulmod_reciprocal_65_129 = 448%nat.
 Proof. static_check. Qed.
 
 Example reciprocal_65_129_max_denominator_bits :
   Bar.max_denominator_bits Bar.mulmod_reciprocal_65_129 = 129%nat.
+Proof. static_check. Qed.
+
+Example reciprocal_65_129_post_product_bit_shift :
+  Bar.post_product_bit_shift Bar.mulmod_reciprocal_65_129 = 0%nat.
 Proof. static_check. Qed.
 
 Example reciprocal_129_193_bits :
@@ -164,12 +192,20 @@ Example reciprocal_129_193_max_denominator_bits :
   Bar.max_denominator_bits Bar.mulmod_reciprocal_129_193 = 193%nat.
 Proof. static_check. Qed.
 
+Example reciprocal_129_193_post_product_bit_shift :
+  Bar.post_product_bit_shift Bar.mulmod_reciprocal_129_193 = 0%nat.
+Proof. static_check. Qed.
+
 Example reciprocal_193_256_bits :
   Bar.reciprocal_bits Bar.mulmod_reciprocal_193_256 = 320%nat.
 Proof. static_check. Qed.
 
 Example reciprocal_193_256_max_denominator_bits :
   Bar.max_denominator_bits Bar.mulmod_reciprocal_193_256 = 256%nat.
+Proof. static_check. Qed.
+
+Example reciprocal_193_256_post_product_bit_shift :
+  Bar.post_product_bit_shift Bar.mulmod_reciprocal_193_256 = 0%nat.
 Proof. static_check. Qed.
 
 Example reciprocal_bits :
@@ -184,6 +220,10 @@ Example reciprocal_pre_product_word_shift :
   Bar.pre_product_word_shift Bar.mulmod_reciprocal = 0%nat.
 Proof. static_check. Qed.
 
+Example reciprocal_post_product_bit_shift :
+  Bar.post_product_bit_shift Bar.mulmod_reciprocal = 0%nat.
+Proof. static_check. Qed.
+
 End Mulmod.
 
 Module MulmodConst.
@@ -196,12 +236,28 @@ Example reciprocal_1_65_max_denominator_bits :
   Bar.max_denominator_bits Bar.mulmod_const_reciprocal_1_65 = 65%nat.
 Proof. static_check. Qed.
 
+Example reciprocal_1_65_bit_shift :
+  Bar.bit_shift Bar.mulmod_const_reciprocal_1_65 = 0%nat.
+Proof. static_check. Qed.
+
+Example reciprocal_1_65_post_product_bit_shift :
+  Bar.post_product_bit_shift Bar.mulmod_const_reciprocal_1_65 = 0%nat.
+Proof. static_check. Qed.
+
 Example reciprocal_65_129_bits :
   Bar.reciprocal_bits Bar.mulmod_const_reciprocal_65_129 = 447%nat.
 Proof. static_check. Qed.
 
 Example reciprocal_65_129_max_denominator_bits :
   Bar.max_denominator_bits Bar.mulmod_const_reciprocal_65_129 = 129%nat.
+Proof. static_check. Qed.
+
+Example reciprocal_65_129_bit_shift :
+  Bar.bit_shift Bar.mulmod_const_reciprocal_65_129 = 0%nat.
+Proof. static_check. Qed.
+
+Example reciprocal_65_129_post_product_bit_shift :
+  Bar.post_product_bit_shift Bar.mulmod_const_reciprocal_65_129 = 0%nat.
 Proof. static_check. Qed.
 
 Example reciprocal_129_193_bits :
@@ -212,12 +268,28 @@ Example reciprocal_129_193_max_denominator_bits :
   Bar.max_denominator_bits Bar.mulmod_const_reciprocal_129_193 = 193%nat.
 Proof. static_check. Qed.
 
+Example reciprocal_129_193_bit_shift :
+  Bar.bit_shift Bar.mulmod_const_reciprocal_129_193 = 0%nat.
+Proof. static_check. Qed.
+
+Example reciprocal_129_193_post_product_bit_shift :
+  Bar.post_product_bit_shift Bar.mulmod_const_reciprocal_129_193 = 0%nat.
+Proof. static_check. Qed.
+
 Example reciprocal_193_256_bits :
   Bar.reciprocal_bits Bar.mulmod_const_reciprocal_193_256 = 319%nat.
 Proof. static_check. Qed.
 
 Example reciprocal_193_256_max_denominator_bits :
   Bar.max_denominator_bits Bar.mulmod_const_reciprocal_193_256 = 256%nat.
+Proof. static_check. Qed.
+
+Example reciprocal_193_256_bit_shift :
+  Bar.bit_shift Bar.mulmod_const_reciprocal_193_256 = 0%nat.
+Proof. static_check. Qed.
+
+Example reciprocal_193_256_post_product_bit_shift :
+  Bar.post_product_bit_shift Bar.mulmod_const_reciprocal_193_256 = 0%nat.
 Proof. static_check. Qed.
 
 Example reciprocal_bits :
@@ -230,6 +302,14 @@ Proof. static_check. Qed.
 
 Example reciprocal_pre_product_word_shift :
   Bar.pre_product_word_shift Bar.mulmod_const_reciprocal = 0%nat.
+Proof. static_check. Qed.
+
+Example reciprocal_bit_shift :
+  Bar.bit_shift Bar.mulmod_const_reciprocal = 0%nat.
+Proof. static_check. Qed.
+
+Example reciprocal_post_product_bit_shift :
+  Bar.post_product_bit_shift Bar.mulmod_const_reciprocal = 0%nat.
 Proof. static_check. Qed.
 
 End MulmodConst.
